\section{Fourier Transforms on the Line} \label{sec:6}

\subsection{The Fourier Transform and the Riemann-Lebesgue Lemma} \label{subsec:6.1}
So far, we have looked at functions $f \in L^1(\T)$, which are 
$2\pi$-periodic, measurable, and integrable on $\R$. We studied their 
Fourier coefficients $(\hat f(n))_{n\in\Z} \in c_0(\Z)$, and the 
``reconstruction'' problem of recovering $f$ from ${\cal F}f = 
(\hat f(n))_{n\in\Z}$.

But what happens if $f$ is not periodic? For example, what if 
$f \in L^1(\R)$ or $f \in L^2(\R)$? Can we still represent $f$ as a 
``sum'' of complex exponentials $x \mapsto e^{inx}$ for $x \in \R$? 

There is now a big issue: the functions $x \mapsto e^{inx}$ no longer 
belong to $L^1(\R)$ or $L^2(\R)$. In particular, the set 
$\{x \mapsto e^{inx} : n \in \Z\}$ no longer forms an orthonormal 
basis for $L^2(\R)$! 

Nonetheless, for all $t \in \R$, the function $x \mapsto e^{itx}$ 
defines a bounded continuous function. So for all $f \in L^1(\R)$, the 
integrals 
\[ \int_{\R} f(x) e^{-itx}\dd x \] 
are well-defined. This leads us to the following definition. 

\begin{defn}{defn:6.1}
    Given $f \in L^1(\R)$, its {\bf Fourier transform} is the function 
    $\hat f : \R \to \C$ given by 
    \[ \hat f(t) = \int_{\R} f(x) e^{-itx}\dd x. \] 
\end{defn}

Up to a scaling factor of $2\pi$, we see that $(\hat f(t))_{t\in\R}$ 
is a continuous analogue of the collection of Fourier coefficients of $f$. 

\begin{exmp}{exmp:6.2}
    Fix $A \in \R$ and let $f = \chi_{[-A, A]}$. Then the Fourier transform 
    of $f$ is 
    \[ \hat f(t) = \int_{-A}^A e^{-itx}\dd x = \frac{1}{-it} e^{-itx} 
    \bigg|_{-A}^A = \frac{e^{iAt} - e^{-iAt}}{it} = \frac{2\sin(At)}{t}. \] 
    Observe that 
    \[ \hat f \in C_0(\R) = \{f : \R \to \C \mid f \text{ continuous and } 
    \textstyle\lim_{t\to\pm\infty} f(t) = 0\}, \] 
    but $\hat f \notin L^1(\R)$. On the other hand, we have $\hat f \in 
    L^2(\R)$ with $\|\hat f\|_2 = 2\pi\|f\|_2$. 
\end{exmp}

Later on, we'll see that these observed properties between $f$ and $\hat f$ 
are in fact generic. We now discuss some basic properties of the Fourier 
transform on $\R$. 

\begin{theo}{theo:6.3}
    Let $f \in L^1(\R)$. Let $\alpha \in \R$ and $\lambda > 0$.
    \begin{enumerate}[(a)]
        \item If $g(x) = f(x)e^{i\alpha x}$, then $\hat g(t) = \hat f(t-\alpha)$. 
        \item If $g(x) = f(x-\alpha)$, then $\hat g(t) = e^{-i\alpha t} \hat f(t)$. 
        \item If $g(x) = \overline{f(-x)}$, then $\hat g(t) = \overline{\hat f(t)}$. 
        \item If $g(x) = f(x/\lambda)$, then $\hat g(t) = \lambda \hat f(\lambda t)$. 
        \item If $g(x) = -ixf(x)$ and $g \in L^1(\R)$, then $\hat f$ is differentiable 
        and $\hat f'(t) = \hat g(t)$. 
    \end{enumerate}    
\end{theo}
\begin{pf}~
    \begin{enumerate}[(a)]
        \item We have 
        \[ \hat g(t) = \int_{\R} f(x) e^{i\alpha x} e^{-itx}\dd x = 
        \int_{\R} f(x) e^{-i(t-\alpha)x}\dd x = \hat f(t - \alpha). \] 
        \item Using the substitution $x \mapsto x + \alpha$, we get 
        \[ \hat g(t) = \int_{\R} f(x-\alpha) e^{-itx}\dd x 
        = \int_{\R} f(x) e^{-it(x+\alpha)}\dd x = e^{-i\alpha t} \hat f(t). \] 
        \item Make the substitution $x \mapsto -x$ to obtain 
        \[ \hat g(t) = \int_{\R} \overline{f(-x)} e^{-itx}\dd x 
        = \overline{\int_{\R} f(-x) e^{itx}\dd x} = 
        \overline{\int_{\R} f(x) e^{-itx}\dd x} = \overline{\hat f(t)}. \] 
        \item Letting $z = x/\lambda$, we get 
        \[ \hat g(t) = \int_{\R} f(x/\lambda) e^{-itx}\dd x 
        = \int_{\R} f(z) e^{-it\lambda z} \dd z 
        = \lambda \int_{\R} f(z) e^{-i(\lambda t)z}\dd z 
        = \lambda \hat f(\lambda t). \] 
        \item Let $(h_n)_{n=1}^\infty \subseteq \R \setminus \{0\}$ be a 
        sequence such that $h_n \to 0$. Then we have 
        \[ \frac{\hat f(t + h_n) - \hat f(t)}{h_n} 
        = \int_{\R} f(x) \left( \frac{e^{-i(t+h_n)x} - e^{-itx}}{h_n} \right) \textrm{d}x 
        = \int_{\R} f(x) e^{-itx} \left( \frac{e^{-ih_nx} - 1}{h_n} \right) \textrm{d}x. \] 
        Set $\varphi_n(x) = (e^{-ih_nx} - 1)/h_n$. It can be seen that 
        for all $x \in \R$, we have $|\varphi_n(x)| \leq |x|$ and 
        $\varphi_n(x) \to -ix$ as $n \to \infty$. This means that 
        \[ |f(x) e^{-itx} \varphi_n(x)| \leq |xf(x)| = |g(x)| \in L^1(\R), \] 
        so by the Dominated Convergence Theorem (Theorem~\ref{theo:2.58}), we get 
        \begin{align*}
            \hat f'(t) 
            &= \lim_{n\to\infty} \frac{\hat f(t + h_n) - \hat f(t)}{h_n} \\
            &= \lim_{n\to\infty} \int_{\R} f(x) e^{-itx} \varphi_n(x)\dd x \\ 
            &= \int_{\R} f(x) e^{-itx} (-ix)\dd x \\ 
            &= \int_{\R} g(x) e^{-itx}\dd x = \hat g(t). \qedhere 
        \end{align*}
    \end{enumerate}
\end{pf}

\begin{theo}[Riemann-Lebesgue Lemma]{theo:6.4}
    Let $f \in L^1(\R)$. Then $\hat f \in C_0(\R)$ and $\|\hat f\|_\infty 
    \leq \|f\|_1$. In particular, if ${\cal F} : L^1(\R) \to C_0(\R)$ 
    denotes the Fourier transform, then ${\cal F}$ is a continuous linear map. 
\end{theo}
\begin{pf}
    Let $f \in L^1(\R)$. Then for all $t \in \R$, we have 
    \[ |\hat f(t)| = \left| \int_{\R} f(x) e^{-itx}\dd x \right| \leq 
    \int_{\R} |f(x)|\dd x = \|f\|_1, \] 
    which tells us that $\|\hat f\|_\infty \leq \|f\|_1$. To see that 
    $\hat f$ is continuous, fix $t \in \R$ and take a sequence $t_n \to t$. 
    Then
    \[ |\hat f(t_n) - \hat f(t)| = \left| \int_{\R} f(x) (e^{-it_nx} - e^{-itx})\dd x \right|. \] 
    Note that $f(x)(e^{-it_nx} - e^{-itx}) \to 0$ pointwise in $x \in \R$ 
    and is dominated by $2|f| \in L^1(\R)$. It follows from the Dominated 
    Convergence Theorem that $|\hat f(t_n) - \hat f(t)| \to 0$ as $n \to \infty$. 

    Finally, to see that $\hat f \in C_0(\R)$, fix $t \neq 0$. We have 
    \begin{align*}
        \hat f(t) &= \int_{\R} f(x) e^{-itx}\dd x \tag{A} \label{eq:5.3} \\ 
        &= -\int_{\R} f(x) e^{i\pi-itx}\dd x \\ 
        &= -\int_{\R} f(x) e^{-it(x-\pi/t)}\dd x \\ 
        &= -\int_{\R} f(z + \pi/t) e^{-itz}\dd z, \tag{B} \label{eq:5.4}
    \end{align*}
    where the last equality was obtained by making the substitution $z = 
    x - \pi/t$. We see that $2\hat f(t)$ can be obtained by 
    adding the results from $\eqref{eq:5.3}$ and $\eqref{eq:5.4}$ together, 
    so we get 
    \[ 2\hat f(t) = \int_{\R} (f(x) - f(x + \pi/t)) e^{-itx}\dd x. \] 
    Note that as $|t| \to \infty$, we have $\pi/t \to 0$. It follows from 
    Exercise 57 of Chapter 18 in Carothers (which we proved on Assignment 4)
    that 
    \[ |2\hat f(t)| \leq \int_{\R} |f(x) - f(x + \pi/t)|\dd x \to 0. \qedhere \] 
\end{pf}

\subsection{Convolutions in $L^1(\R)$} \label{subsec:6.2}
The story here is essentially identical to that of $L^1(\T)$ and our 
study of convolution there. For the moment, let $f, g \in C_c(\R)$, 
and note that $C_c(\R) \subseteq L^1(\R) \cap L^2(\R) \cap L^\infty(\R)$.
We define $f \star g : \R \to \C$ by 
\begin{align*}
    (f \star g)(x) &= \int_{\R} f(y)g(x - y)\dd y 
    = \int_{\R} f(-y) g(x+y) \dd y 
    = \int_{\R} f(x-y) g(y) \dd y = (g \star f)(x), 
\end{align*}
where we made the substitutions $y \mapsto -y$ and $y \mapsto x+y$ above. 
Note that $f \star g = g \star f$ is also well-defined in the case where 
$f \in L^\infty(\R)$ and $g \in L^1(\R)$, or when both $f, g \in L^2(\R)$. 

\begin{prop}{prop:6.5}
    Let $f, g \in C_c(\R)$. Then 
    \begin{enumerate}[(1)]
        \item $f \star g = g \star f \in C_c(\R)$; 
        \item $\|f \star g\|_p \leq \|f\|_p \|g\|_1$ for $p = 1, 2, \infty$; and 
        \item $\|f \star g\|_\infty \leq \|f\|_2 \|g\|_2$. 
    \end{enumerate}
\end{prop}

We'll omit the proof of (2) as it is identical to the proofs of the 
statements for $L^1(\T)$ from Proposition~\ref{prop:5.1}. The proof 
was based on the uniform continuity of $f \in C(\T)$, and one can 
repeat the argument for $f \in C_c(\R)$ as well because $f$ is then 
uniformly continuous on $\R$. 

To prove (1) and (3), we'll first need a lemma. 

\begin{lemma}{lemma:6.6}
    Given $f : \R \to \C$ and $y \in \R$, let $f_y(x) = f(x-y)$. 
    If $f \in L^p(\R)$, then the map $y \mapsto f_y$ is uniformly 
    continuous as a map $\R \to L^p(\R)$ for all $p \in [1, \infty)$. 
    That is, for all $\eps > 0$, there exists $\delta > 0$ such that 
    $|s - t| < \delta$ implies $\|f_s - f_t\|_p < \eps$. 
\end{lemma}
\begin{pf}
    Let $\eps > 0$. Let $f \in L^p(\R)$ for $p \in [1, \infty)$, and choose 
    $g \in C_c(\R)$ such that $\|f - g\|_p < \eps$. Assume that 
    $\text{supp}(g) \subseteq [-A, A]$ for some $A > 0$. 
    By the uniform continuity of $g$, there exists $0 < \delta < A$ 
    such that $|g(s) - g(t)| < \eps$ whenever $|s - t| < \delta$. Then we 
    have 
    \[ \|g_s - g_t\|_p^p = \int_{\R} |g(x-s) - g(x-t)|^p\dd x 
    < \eps^p \int_{\text{supp}(g_s-g_t)} 1\dd x \leq \eps^p(2A + \delta) 
    < 3A \eps^p. \] 
    Since $\|\cdot\|_p$ is translation invariant, it follows that 
    \begin{align*}
        \|f_s - f_t\|_p &\leq \|f_s - g_s\|_p + \|g_s - g_t\|_p 
        + \|g_t - f_t\|_p \\ 
        &= \|f - g\|_p + \|g_s - g_t\|_p + \|f - g\|_p \\ 
        &< 2\eps + (3A)^{1/p} \eps. \qedhere 
    \end{align*} 
\end{pf}

{\sc Proof of Proposition~\ref{prop:6.5}.} Let $f, g \in C_c(\R)$. 
Note that when $|x|$ is large, we have 
\[ (f \star g)(x) = \int_{\R} f(y) g(x-y)\dd y = 0, \] 
because eventually the support of $f$ and the support of $y \mapsto g(x-y)$ 
will not overlap. That is, $f \star g$ is compactly supported. So if we 
can establish continuity, then $f \star g \in C_c(\R)$. 

Put $\check g(y) = g(-y)$. Then we see that 
\[ (f \star g)(x) = \int_{\R} f(y) g(x-y)\dd y = \int_{\R} 
f(y) \check g(y-x)\dd y = \langle \check g_x, \overline f \rangle_{L^2(\R)}. \] 
Now, suppose that $x \to x_0 \in \R$. Using Cauchy-Schwarz and 
Lemma~\ref{lemma:6.6}, we get 
\begin{align*}
    |(f \star g)(x) - (f \star g)(x_0)| 
    &= |\langle \check g_x - \check g_{x_0}, \overline f \rangle| \\
    &\leq \| \check g_x - \check g_{x_0} \|_2 \| \overline f \|_2 \to 0. 
\end{align*}
Thus, $f \star g$ is continuous and $f \star g \in C_c(\R)$. 
Moreover, for all $x \in \R$, we see from Cauchy-Schwarz that
\[ |(f \star g)(x)| = |\langle \check g_x, \overline f \rangle_{L^2(\R)}|
\leq \|\check g_x\|_2 \|\overline f\|_2 = \|g\|_2 \|f\|_2, \] 
so $\|f \star g\|_\infty \leq \|g\|_2 \|f\|_2$. \qed 

We know that $C_c(\R)$ is dense in $L^p(\R)$ for $p \in [1, \infty)$. 
Then the inequality $\|f \star g\|_1 \leq \|f\|_1 \|g\|_1$ together 
with density tells us that $f \star g$ makes sense for $f, g \in L^1(\R)$. 
In particular, we can continuously extend convolution to $L^1(\R)$, 
and $L^1(\R)$ is an algebra under convolution!  

Moreover, the inequality $\|f \star g\|_\infty \leq \|f\|_2 \|g\|_2$ 
implies that $f \star g$ is well-defined for $f, g \in L^2(\R)$ and 
$f \star g \in C_0(\R)$. Indeed, one can take sequences $f_n \to f$ 
and $g_n \to g$, then show that $f \star g$ is the uniform limit of 
$f_n \star g_n$ with an argument similar to that of Theorem~\ref{theo:5.3}.

\begin{prop}{prop:6.7}
    The Fourier transform ${\cal F} : L^1(\R) \to C_0(\R)$ which 
    maps $f \in L^1(\R)$ to ${\cal F}f = (\hat f(t))_{t\in\R}$ given by 
    \[ \hat f(t) = \int_{\R} f(x) e^{-itx}\dd x \] 
    is an algebra homomorphism. That is, for any $f, g \in L^1(\R)$, 
    we have ${\cal F}(f \star g) = {\cal F}(f) {\cal F}(g) \in C_0(\R)$. 
\end{prop}
\begin{pf}
    By the density of $C_c(\R)$ in $L^1(\R)$ and the continuity of ${\cal F} : 
    L^1(\R) \to C_0(\R)$, it suffices to prove this for $f, g \in C_c(\R)$. 
    In this case, we have for all $t \in \R$ that 
    \begin{align*}
        (\widehat{f \star g})(t) 
        &= \int_{\R} \left( \int_{\R} f(y)g(x-y)\dd y \right) e^{-itx}\dd x \\ 
        &= \int_{\R} \int_{\R} f(y) g(x-y) e^{-itx}\dd x \dd y \\ 
        &= \int_{\R} f(y) e^{-ity} \hat g(t) \dd y = \hat f(t) \hat g(t),
    \end{align*}
    where we applied Fubini for the second equality. 
\end{pf}

\subsection{Fourier Inversion Theorem} \label{subsec:6.3}
Let $f \in L^1(\R)$. 
\begin{enumerate}[(1)]
    \item Is $f$ uniquely determined by its Fourier transform 
    ${\cal F}f = (\hat f(t))_{t\in\R}$? That is, if $\hat f(t) = \hat g(t)$
    for all $t \in \R$, then do we have $f = g$ almost everywhere? 
    Equivalently, is ${\cal F} : L^1(\R) \to C_0(\R)$ injective? 
    \item If the answer to the previous question is yes, then how do we reconstruct 
    $f$ from $\hat f$? 
\end{enumerate}
Recall that if $f \in L^1(\T)$ and we assume moreover that $\hat f = 
(\hat f(n))_{n\in\Z} \in \ell^1(\Z)$ (a strong assumption), then we know 
from our study of Fourier series that 
\[ g(x) = \sum_{n\in\Z} \hat f(n) e^{inx} \] 
converges absolutely for $x \in [-\pi, \pi]$ and $f = g$ almost everywhere. 
In this special situation, $f$ is recovered almost everywhere by simply 
summing the Fourier series of $f$!

For the Fourier transform on $\R$, the ``continuous'' version of the above holds. 
This is the Fourier inversion theorem on $L^1(\R)$. 

\begin{theo}[Fourier Inversion Theorem on $L^1(\R)$]{theo:6.8}
    Let $f \in L^1(\R)$, and assume that $\hat f \in L^1(\R)$ as well. Define 
    \[ g(x) = \frac{1}{2\pi} \int_{\R} \hat f(t) e^{itx}\dd t. \] 
    Then $g \in C_0(\R)$ and $g = f$ almost everywhere. That is, for 
    almost every $x \in \R$, we have 
    \[ f(x) = \frac{1}{2\pi} \int_{\R} \hat f(t) e^{itx}\dd t. \]
\end{theo}

As an immediate consequence, we get an affirmative answer to our first 
question above. 

\begin{cor}{cor:6.9}
    The Fourier transform ${\cal F} : L^1(\R) \to C_0(\R)$ is injective.
\end{cor}
\begin{pf}
    If $f, g \in L^1(\R)$ satisfies $\hat f = \hat g$, then 
    $\widehat{f-g} = 0 \in L^1(\R)$. It follows from the Fourier inversion 
    theorem (Theorem~\ref{theo:6.8}) that 
    \[ (f - g)(x) = \frac{1}{2\pi} \int_{\R} 0 e^{itx}\dd x = 0 \] 
    for almost every $x \in \R$, so $f = g$ almost everywhere. 
\end{pf}

The second question is partially answered by the Fourier inversion theorem. 
During the proof, we will develop a technique involving Ces\`aro summation 
and summability kernels that will fully answer the second question. 

Before we get to the proof, let's see why the theorem should hold heuristically 
by giving an engineer's ``proof''. Assume that $f \in L^1(\R)$ is bounded 
and continuous, and for $A > 0$, set $f_A = f\chi_{[-A, A]}$. Then 
we have $\lim_{A\to\infty} f_A = f$ in $L^1(\R)$. If we regard $f_A$ as a
$2\pi A$-periodic function, then $f_A$ has Fourier series 
\[ \sum_{n\in\Z} c_n e^{i(n/A)x}, \] 
where the coefficients $c_n$ are 
\[ c_n = \frac{1}{2\pi A} \int_{-\pi A}^{\pi A} f_A(x) e^{-i(n/A)x} \dd x 
= \frac{1}{2\pi A} \hat f_A(n/A). \] 
Moreover, if $f$ is sufficiently nice (for example, $f \in C^1(\R)$), then 
\[ f_A(x) = \sum_{n\in\Z} c_n e^{i(n/A)x} = \frac{1}{2\pi} 
\sum_{n\in\Z} \frac{1}{A} \hat f_A(n/A) e^{i(n/A)x}. \] 
This is a Riemann sum with respect to an infinite partition of $\R$ 
with common width $1/A$ and boundary points $n/A$ for $n \in \Z$. 
Then as $A \to \infty$, we have 
\[ \frac{1}{2\pi} \sum_{n\in\Z} \frac{1}{A} \hat f_A(n/A) e^{i(n/A)x} 
\to \frac{1}{2\pi} \int_{\R} \hat f(t) e^{itx}\dd t. \] 
We saw above that $f_A \to f$, so we get 
\[ f(x) = \frac{1}{2\pi} \int_{\R} \hat f(t) e^{itx}\dd t. \] 
Of course, this is all mathematical nonsense, and we are assuming far 
too many conditions on our function $f \in L^1(\R)$. To make this rigorous, 
we will need to take a more devious approach. 

We start with a pair of functions where the Fourier inversion theorem 
can be verified directly. Let $H(t) = e^{-|t|}$. For $\lambda > 0$, 
set $H_\lambda(t) = H(\lambda t) = e^{-\lambda|t|}$, and define 
\[ h_\lambda(x) = \frac{1}{2\pi} \int_{\R} H_\lambda(t) e^{itx}\dd x. \] 

\begin{lemma}{lemma:6.10}
    For all $x \in \R$, we have 
    \[ h_\lambda(x) = \frac{\lambda}{\pi} \cdot \frac{1}{x^2 + \lambda^2}. \] 
\end{lemma}
\begin{pf}
    By directly computing the integral, we get 
    \begin{align*}
        h_{\lambda}(x) &= \frac{1}{2\pi} \int_{\R} e^{-\lambda|t|+itx}\dd t \\ 
        &= \frac{1}{2\pi} \left( \int_0^\infty e^{(-\lambda+ix)t}\dd t 
        + \int_{-\infty}^0 e^{(\lambda+ix)t} \dd t \right) \\ 
        &= \frac{1}{2\pi} \left( \frac{1}{-\lambda+ix} (-1) + \frac{1}{\lambda+ix} \right) \\ 
        &= \frac{1}{2\pi} \left( \frac{-(\lambda + ix) + (-\lambda+ix)}{-x^2-\lambda^2} \right) \\ 
        &= \frac{1}{2\pi} \cdot \frac{-2\lambda}{-x^2-\lambda^2} \\
        &= \frac{\lambda}{\pi} \cdot \frac{1}{x^2+\lambda^2}. \qedhere 
    \end{align*}
\end{pf}
Here, we see that $0 \leq H_\lambda(t) \leq 1$ and $H_\lambda(t) \to 1$ 
as $t \to 0$. Moreover, we have $h_\lambda \geq 0$ and 
\[ \|h_\lambda\|_1 = \int_{\R} h_\lambda(x) \dd x = 
\frac{1}{\pi} \lim_{R\to0} \int_{-R}^R \frac{1}{\lambda} \cdot 
\frac{1}{1 + (x/\lambda)^2}\dd x = \frac{1}{\pi} \lim_{R\to0} 
\arctan(x/\lambda) \bigg|_{-R}^R = 1. \] 
The following theorem shows us that $(h_\lambda)_{\lambda > 0}$ acts like a 
summability kernel for the Fourier transform. 

\begin{theo}{theo:6.11}
    Let $p \in [1, \infty)$. If $f \in L^p(\R)$, then 
    $\|f \star h_\lambda - f\|_p \to 0$ as $\lambda \to 0$. Moreover, if 
    $f$ is continuous at $x \in \R$ and $\|f\|_\infty < \infty$, then 
    \[ f(x) = \lim_{\lambda\to 0} (f \star h_\lambda)(x). \] 
\end{theo}
\begin{pf}
    Suppose that $f$ is continuous at $x \in \R$, and $\|f\|_\infty < \infty$. 
    Using the fact that $\|h_\lambda\|_1 = 1$ and the substitution 
    $s = y/\lambda$, we have  
    \begin{align*}
        |(f \star h_\lambda)(x) - f(x)| 
        &= \left| \int_{\R} (f(x-y) - f(x)) h_\lambda(y)\dd y \right| \\
        &\leq \int_{\R} |f(x-y) - f(x)| h_\lambda(y) \dd y \\ 
        &= \int_{\R} |f(x-y) - f(x)| \lambda h_1(y/\lambda) \dd y \\ 
        &= \int_{\R} |f(x-\lambda s) - f(x)| h_1(s)\dd s. 
    \end{align*}
    We have a bound on the integrand given by 
    \[ |f(x-\lambda s) - f(x)| h_1(s) \leq 2\|f\|_\infty h_1(s). \] 
    Moreover, by taking a sequence $\lambda_n \to 0$, we see that 
    \[ |f(x - \lambda_n s) - f(x)| h_1(s) \to 0 \] 
    since $f$ is continuous. It follows from the Dominated Convergence 
    Theorem that 
    \[ |(f \star h_\lambda)(x) - f(x)| \to 0. \] 
    We now prove the first part of the theorem. Let $\eps > 0$, 
    and choose $f_0 \in C_c(\R)$ such that $\|f - f_0\|_p < \eps$. Then 
    \[ \|f \star h_\lambda - f\|_p \leq 
    \|f \star h_\lambda - f_0 \star h_\lambda\|_p + \|f_0 \star h_\lambda 
    - f_0\|_p + \|f_0 - f\|_p < 2\eps + \|f_0 \star h_\lambda - f_0\|_p, \] 
    so it suffices to prove this for $f = f_0 \in C_c(\R)$ by density. 
    First, we have 
    \begin{align*}
        \|f \star h_\lambda - f\|_p^p 
        &= \int_{\R} \left| \int_{\R} (f(x-y) - f(x)) h_\lambda(y) \dd y 
        \right|^p \textrm{d}x \\ 
        &\leq \int_{\R} \int_{\R} |f(x-y) - f(x)|^p h_\lambda(y)\dd y \dd x. 
    \end{align*}
    The inequality is clear for $p = 1$. For $p = 2$, this is obtained by 
    applying Cauchy-Schwarz to the pair $y \mapsto (f(x-y) - f(x))(h_\lambda(y))^{1/2}$ 
    and $(h_\lambda(y))^{1/2}$, and using the fact that $\|h_\lambda\|_1 = 1$. 
    Next, by Fubini and the substitution $s = y/\lambda$, we have 
    \begin{align*}
        \|f \star h_\lambda - f\|_p^p 
        &\leq \int_{\R} \int_{\R} |f(x-y) - f(x)|^p h_\lambda(y)\dd y \dd x \\ 
        &= \int_{\R} \left( \int_{\R} |f(x-y) - f(x)|^p \dd x \right) h_\lambda(y) \dd y \\ 
        &= \int_{\R} \|f_y - f\|_p^p h_\lambda(y)\dd y \\ 
        &= \int_{\R} \|f_{\lambda s} - f\|_p^p h_1(s)\dd s. 
    \end{align*}
    Similar to the argument above, we have 
    \[ \|f_{\lambda s} - f\|_p^p h_1(s) \leq 2^p \|f\|_p h_1(s) \] 
    and taking a sequence $\lambda_n \to 0$ gives us
    \[ \|f_{\lambda_n s} - f\|_p^p h_1(s) \to 0, \] 
    so it follows from the Dominated Convergence Theorem that 
    \[ \|f \star h_\lambda - f\|_p^p \to 0. \qedhere \] 
\end{pf}

The following lemma is an approximate version of the Fourier inversion theorem 
in view of Theorem~\ref{theo:6.11}, noting that $H_\lambda \approx 1$ and 
$f \star h_\lambda \approx f$. 

\begin{lemma}{lemma:6.12}
    If $f \in L^1(\R)$, then for all $\lambda > 0$ and $x \in \R$, we have 
    \[ (f \star h_\lambda)(x) = \frac{1}{2\pi} \int_{\R} H_\lambda(t) 
    \hat f(t) e^{itx}\dd x. \] 
\end{lemma}
\begin{pf}
    Let $f \in L^1(\R)$. Then we have 
    \begin{align*}
        (f \star h_\lambda)(x) 
        &= \frac{1}{2\pi} \int_{\R} f(x-y) \int_{\R} H_\lambda(t) e^{ity} \dd t \dd y \\ 
        &= \frac{1}{2\pi} \int_{\R} \int_{\R} f(x-y) H_\lambda(t) e^{ity} \dd y \dd t \\ 
        &= \frac{1}{2\pi} \int_{\R} \int_{\R} f(z) H_\lambda(t) e^{it(x-z)} \dd z \dd t \\ 
        &= \frac{1}{2\pi} \int_{\R} \hat f(t) H_\lambda(t) e^{itx} \dd t, 
    \end{align*}
    where we used Fubini for the second equality and the substitution 
    $z = x - y$ for the third equality. 
    
    \newpage 
    However, we note that the use of Fubini here was not fully rigorous, 
    as Fubini applies to integrals over compact intervals. To fix this, 
    we can take a sequence $f_n \in C_c(\R)$ with $f_n \to f$ in $L^1(\R)$. 
    Then we have $(f \star h_\lambda)(x) = \lim_{n\to\infty} (f_n \star 
    h_\lambda)(x)$. Also, we see that 
    \begin{align*}
        (f_n \star h_\lambda)(x) 
        &= \frac{1}{2\pi} \int_{\R} f_n(x-y) \lim_{N\to\infty} \int_{-N}^N H_\lambda(t) e^{ity} \dd t \dd y \\ 
        &= \lim_{N\to\infty} \frac{1}{2\pi} \int_{\R} f_n(x-y) \int_{-N}^N H_\lambda(t) e^{ity} \dd t \dd y \\
        &= \lim_{N\to\infty} \int_{-N}^N H_\lambda(t) \frac{1}{2\pi} \int_{\R} f_n(x-y) e^{ity} \dd y \dd t \\ 
        &= \lim_{N\to\infty} \frac{1}{2\pi} \int_{-N}^N H_\lambda(t) \hat f_n(t) e^{itx} \dd t \\ 
        &= \frac{1}{2\pi} \int_{\R} H_\lambda(t) \hat f_n(t) e^{itx} \dd t,
    \end{align*}
    where the second and final equalities were obtained by the Dominated Convergence 
    Theorem. Then the continuity of ${\cal F} : L^1(\R) \to C_0(\R)$ tells us that 
    as $n \to \infty$, we have 
    \[ (f_n \star h_\lambda)(x) 
    = \frac{1}{2\pi} \int_{\R} H_\lambda(t) \hat f_n(t) e^{itx} \dd t
    \to \frac{1}{2\pi} \int_{\R} H_\lambda(t) \hat f(t) e^{itx} \dd t. \qedhere \] 
\end{pf}

With all these tools, the Fourier inversion theorem follows quickly. 

{\sc Proof of Theorem~\ref{theo:6.8}.} Suppose that $f \in L^1(\R)$ with 
$\hat f \in L^1(\R)$ as well. Take a sequence $\lambda_n \to 0$. 
Note that $H_{\lambda_n}(t) \hat f(t) e^{itx} \to \hat f(t) e^{itx}$ 
as $\lambda_n \to 0$, and that this is bounded above by $|\hat f| \in L^1(\R)$. 
Then by Lemma~\ref{lemma:6.12} and the Dominated Convergence Theorem, we have 
\[ (f \star h_{\lambda_n})(x) = \frac{1}{2\pi} \int_{\R} H_{\lambda_n}(t) 
\hat f(t) e^{itx} \dd x \to \frac{1}{2\pi} \int_{\R} \hat f(t) e^{itx} \dd x = g(x). \]
We also know that $f = \lim_{n\to\infty} f \star h_{\lambda_n}$, so 
we have $f = \lim_{n\to\infty} f \star h_{\lambda_n} = g$ pointwise 
almost everywhere. \qed 
